logic/logic_aux_lemmas.v
@@ -7,348 +7,6 @@ Add LoadPath "E:\Ziga_Podatki\faks\eeff-formalization\substitution".
 
 Require Export subtyping_lemmas.
 
-(* 
-Lemma heq_cases_ceq Σ D Γ Ψ h1 h2 op A B c1 c2 :
-  judg Γ Ψ (Heq Σ D h1 h2) -> get_op_type Σ op = Some (A, B) ->
-  get_case h1 op = Some c1 ->
-  get_case h2 op = Some c2 ->
-  judg (CtxU (CtxU Γ A) (TyFun B D)) (hyp_shift Ψ 2 0) (Ceq D c1 c2).
-Proof.
-intros eqs gets finds1 finds2.
-induction Σ. simpl in gets. discriminate.
-simpl in *. destruct (op==o).
-+ inv gets. inv eqs. inv H1.
-  rewrite H8 in finds1. rewrite H12 in finds2.
-  inv finds1. inv finds2. auto.
-+ inv eqs. inv H1. eauto.
-Qed. *)
-
-(* ==================== Logic Subtyping ==================== *)
-(* 
-Lemma heq_subtype Σ Σ' D Γ Ψ h1 h2 (orig : judg Γ Ψ (Heq Σ D h1 h2)) :
-  wf_sig Σ' -> sig_subtype Σ' Σ -> judg Γ Ψ (Heq Σ' D h1 h2).
-Proof.
-intros wf sty. induction Σ' as [ | Σ' IH o A' B'].
-+ inv orig. inv H. eapply WfJudg; auto.
-  eapply WfHeq. 4: exact H10. 4: exact H11. auto.
-  apply SubtypeSigØ. apply SubtypeSigØ. apply HeqSigØ.
-+ inv orig. inv H. eapply WfJudg; auto.
-  eapply WfHeq. auto. 3: exact H10. 3: exact H11.
-  { eapply sig_subtype_trans; eauto. }
-  { eapply sig_subtype_trans; eauto. }
-  inv sty. inv wf.
-  eapply sig_subtype_get_Some in H8 as g1; eauto.
-  eapply sig_subtype_get_Some in H9 as g2; eauto.
-  destruct g1 as [A1[B1[get1[_ _]]]].
-  destruct g2 as [A2[B2[get2[_ _]]]].
-  eapply h_has_case in H10 as case1; eauto.
-  eapply h_has_case in H11 as case2; eauto.
-  destruct case1 as [c1 find1].
-  destruct case2 as [c2 find2].
-  clear A1 B1 get1 A2 B2 get2.
-  eapply HeqSigU; eauto.
-  assert 
-    (judg (CtxU (CtxU Γ A'0) (TyFun B'0 D)) (hyp_shift Ψ 2 0) (Ceq D c1 c2)).
-  - eapply heq_cases_ceq. 2: eauto. all: eauto.
-    eapply WfJudg; eauto. eapply WfHeq. 2: exact H8. all: eauto.
-  - eapply ctx_subtype_judg; eauto.
-    * inv H10. apply WfCtxU. apply WfCtxU. 3: apply WfTyFun. all: auto.
-    * apply SubtypeCtxU. apply SubtypeCtxU. 3: apply SubtypeTyFun. all: auto.
-      all: inv H10; (apply ctx_subtype_refl || apply csubtype_refl); auto.
-Qed. *)
-
-(* This formulation is needed so that the termination
-   checker doesnt run forever. *)
-(* Fixpoint veq_subtype Γ Ψ φ (orig: judg Γ Ψ φ) A A' v1 v2 {struct orig} :
-  φ = Veq A v1 v2 ->
-  wf_vtype A' -> vsubtype A A' -> 
-  judg Γ Ψ (Veq A' v1 v2)
-with ceq_subtype Γ Ψ φ (orig: judg Γ Ψ φ) C C' c1 c2 {struct orig} :
-  φ = Ceq C c1 c2 ->
-  wf_ctype C' -> csubtype C C' -> 
-  judg Γ Ψ (Ceq C' c1 c2).
-Proof.
-{ 
-intros same wfa' stya.
-assert (wf_ctx Γ) as wfctx.
-{ clear veq_subtype ceq_subtype. inv orig. inv H. inv H5. auto. } 
-assert (has_vtype Γ v1 A') as ty1.
-{ clear veq_subtype ceq_subtype. inv orig. inv H.
-  apply TypeV; auto. eapply TypeVSubtype; eauto. }
-assert (has_vtype Γ v2 A') as ty2.
-{ clear veq_subtype ceq_subtype. inv orig. inv H.
-  apply TypeV; auto. eapply TypeVSubtype; eauto. }
-apply WfJudg; auto. apply WfVeq; auto.
-{ clear veq_subtype ceq_subtype. inv orig. auto. }
-destruct orig. destruct H1; inv same.
-+ specialize (veq_subtype _ _ _ H1) as IH.
-  clear veq_subtype ceq_subtype.
-  apply VeqSym. eauto.
-+ specialize (veq_subtype _ _ _ H1) as IH1.
-  specialize (veq_subtype _ _ _ H2) as IH2.
-  clear veq_subtype ceq_subtype.
-  eapply VeqTrans; eauto.
-+ clear veq_subtype ceq_subtype.
-  eapply VeqVar; eauto. eapply vsubtype_trans; eauto.
-+ clear veq_subtype ceq_subtype. 
-  inv stya. apply VeqUnit; eauto.
-+ clear veq_subtype ceq_subtype. 
-  inv stya. apply VeqInt; eauto.
-+ inv stya.
-  specialize (veq_subtype _ _ _ H1) as IH1.
-  specialize (veq_subtype _ _ _ H2) as IH2.
-  clear veq_subtype ceq_subtype.
-  inv wfa'. eapply VeqPair; eauto.
-+ inv stya. 
-  specialize (veq_subtype _ _ _ H1) as IH.
-  clear veq_subtype ceq_subtype.
-  inv wfa'. eapply VeqInl; eauto.
-+ inv stya.
-  specialize (veq_subtype _ _ _ H1) as IH.
-  clear veq_subtype ceq_subtype.
-  inv wfa'. eapply VeqInr; eauto.
-+ clear veq_subtype ceq_subtype. 
-  inv stya. eapply VeqListNil.
-+ inv stya. 
-  specialize (veq_subtype _ _ _ H1) as IH1.
-  specialize (veq_subtype _ _ _ H2) as IH2.
-  clear veq_subtype ceq_subtype.
-  inv wfa'. eapply VeqListCons; eauto.
-  eapply IH2. eauto.
-  apply WfTyList. auto. 
-  apply SubtypeTyList. auto.
-+ inv stya.
-  specialize (ceq_subtype _ _ _ H1) as IH.
-  clear veq_subtype ceq_subtype.
-  inv wfa'. apply VeqFun.
-  eapply ctx_subtype_judg. eauto.
-  - apply WfCtxU; auto.
-  - apply SubtypeCtxU; auto. apply ctx_subtype_refl. auto.
-+ inv stya.
-  specialize (ceq_subtype _ _ _ H1) as IH.
-  clear veq_subtype ceq_subtype.
-  inv wfa'. inv H6. inv H7. eapply VeqHandler.
-  eapply ctx_subtype_judg. eauto.
-  - apply WfCtxU; auto.
-  - apply SubtypeCtxU; auto. apply ctx_subtype_refl. auto.
-  - eapply heq_subtype; eauto.
-  - eapply csubtype_trans; eauto.
-+ clear veq_subtype ceq_subtype. inv stya. apply ηUnit.
-+ clear veq_subtype ceq_subtype. inv stya. apply ηFun.
-}{
-intros same wfc' styc.
-assert (wf_ctx Γ) as wfctx.
-{ clear veq_subtype ceq_subtype. inv orig. inv H. inv H5. auto. } 
-assert (has_ctype Γ c1 C') as ty1.
-{ clear veq_subtype ceq_subtype. inv orig. inv H.
-  apply TypeC; auto. eapply TypeCSubtype; eauto. }
-assert (has_ctype Γ c2 C') as ty2.
-{ clear veq_subtype ceq_subtype. inv orig. inv H.
-  apply TypeC; auto. eapply TypeCSubtype; eauto. }
-apply WfJudg; auto. apply WfCeq; auto.
-{ clear veq_subtype ceq_subtype. inv orig. auto. }
-destruct orig. destruct H1; inv same.
-+ specialize (ceq_subtype _ _ _ H1) as IH.
-  clear veq_subtype ceq_subtype.
-  apply CeqSym. eauto.
-+ specialize (ceq_subtype _ _ _ H1) as IH1.
-  specialize (ceq_subtype _ _ _ H2) as IH2.
-  clear veq_subtype ceq_subtype.
-  eapply CeqTrans; eauto.
-+ inv styc.
-  specialize (veq_subtype _ _ _ H1) as IH.
-  clear veq_subtype ceq_subtype.
-  inv wfc'. eapply CeqRet; eauto.
-+ clear veq_subtype ceq_subtype.
-  eapply CeqAbsurd; eauto.
-+ specialize (ceq_subtype _ _ _ H2) as IH.
-  clear veq_subtype ceq_subtype.
-  eapply CeqΠMatch; eauto.
-+ specialize (ceq_subtype _ _ _ H2) as IH1.
-  specialize (ceq_subtype _ _ _ H3) as IH2.
-  clear veq_subtype ceq_subtype.
-  eapply CeqΣMatch; eauto.
-+ specialize (ceq_subtype _ _ _ H2) as IH1.
-  specialize (ceq_subtype _ _ _ H3) as IH2.
-  clear veq_subtype ceq_subtype.
-  eapply CeqListMatch; eauto.
-+ inv styc. rename A' into B'.
-  specialize (ceq_subtype _ _ _ H1) as IH1.
-  specialize (ceq_subtype _ _ _ H2) as IH2.
-  clear veq_subtype ceq_subtype.
-  assert (wf_vtype A).
-  { inv H1. inv H3. inv H11. inv H3. auto. }
-  eapply CeqDoBind.
-  - eapply IH1. eauto. apply WfCTy; eauto; inv wfc'; auto.
-    apply SubtypeCTy; auto. apply vsubtype_refl. auto.
-  - eapply IH2; eauto. apply SubtypeCTy; auto.
-+ specialize (veq_subtype _ _ _ H1) as IH.
-  clear veq_subtype ceq_subtype.
-  assert (wf_vtype A).
-  { inv H2. inv H3. inv H8. auto. }
-  eapply CeqApp; eauto. eapply IH. eauto.
-  - apply WfTyFun; assumption.
-  - apply SubtypeTyFun. apply vsubtype_refl. all: auto.
-+ rename C' into D'.
-  specialize (veq_subtype _ _ _ H1) as IH.
-  clear veq_subtype ceq_subtype.
-  assert (wf_ctype C0).
-  { inv H1. inv H3. inv H8. inv H3. auto. }
-  eapply CeqHandle; eauto. eapply IH. eauto.
-  - apply WfTyHandler; assumption.
-  - apply SubtypeTyHandler. apply csubtype_refl. all: auto.
-+ rename C' into D'.
-  specialize (ceq_subtype _ _ _ H2) as IH.
-  clear veq_subtype ceq_subtype.
-  eapply CeqLetRec; eauto.
-+ specialize (veq_subtype _ _ _ H2) as IH1.
-  specialize (ceq_subtype _ _ _ H3) as IH2.
-  clear veq_subtype ceq_subtype.
-  inv styc.
-  eapply sig_subtype_get_Some in H9 as getop; eauto.
-  destruct getop as [A_op'[B_op'[gets[asty bsty]]]].
-  eapply CeqOp; eauto; inv wfc'.
-  - eapply IH1. eauto.
-    eapply get_op_type_wf in gets. destruct gets. all: auto.
-  - eapply ctx_subtype_judg; eauto.
-    * eapply IH2. eauto. apply WfCTy; eauto. apply SubtypeCTy; auto.
-    * apply WfCtxU. auto. 
-      eapply get_op_type_wf in gets. destruct gets. all: auto.
-    * eapply SubtypeCtxU. apply ctx_subtype_refl. all: auto.
-+ clear veq_subtype ceq_subtype.
-  inv styc. eapply OOTB; eauto. eapply eqs_subtype_contains; eauto.
-  eapply wf_inst_tctx_subtype; eauto.
-  apply SubtypeCTy; auto.
-+ clear veq_subtype ceq_subtype.
-  eapply βΠMatch.
-+ clear veq_subtype ceq_subtype.
-  eapply βΣMatch_Inl.
-+ clear veq_subtype ceq_subtype.
-  eapply βΣMatch_Inr.
-+ clear veq_subtype ceq_subtype.
-  eapply βListMatch_Nil.
-+ clear veq_subtype ceq_subtype.
-  eapply βListMatch_Cons.
-+ clear veq_subtype ceq_subtype.
-  eapply βApp.
-+ clear veq_subtype ceq_subtype.
-  eapply βLetRec.
-+ clear veq_subtype ceq_subtype.
-  eapply βDoBind_Ret.
-+ clear veq_subtype ceq_subtype.
-  eapply βDoBind_Op.
-+ clear veq_subtype ceq_subtype.
-  eapply βHandle_Ret.
-+ clear veq_subtype ceq_subtype.
-  eapply βHandle_Op. eauto.
-+ clear veq_subtype ceq_subtype.
-  eapply ηPair. omega.
-  apply TypeC. inv H2. eauto. auto. eapply TypeCSubtype; eauto.
-+ clear veq_subtype ceq_subtype.
-  eapply ηSum. omega.
-  apply TypeC. inv H2. eauto. auto. eapply TypeCSubtype; eauto.
-+ clear veq_subtype ceq_subtype.
-  eapply ηList. omega.
-  apply TypeC. inv H2. eauto. auto. eapply TypeCSubtype; eauto.
-+ clear veq_subtype ceq_subtype.
-  eapply ηDoBind.
-}
-Qed. *)
-
-(* ==================== Structural Rules for Cases ==================== *)
-
-(* Lemma heq_case_extend_trivial Σ D Γ Ψ h1 h2 op A1 A2 B1 B2 c1 c2:
-  judg Γ Ψ (Heq Σ D h1 h2) ->
-  get_case h1 op = None -> get_case h2 op = None ->
-  has_ctype (CtxU (CtxU Γ A1) (TyFun B1 D)) c1 D ->
-  has_ctype (CtxU (CtxU Γ A2) (TyFun B2 D)) c2 D ->
-  judg Γ Ψ (Heq Σ D (CasesU h1 op c1) (CasesU h2 op c2)).
-Proof.
-intros orig f1 f2 tys1 tys2.
-assert (wf_vtype A1) as wfa1 by (inv tys1; inv H; inv H4; auto).
-assert (wf_vtype A2) as wfa2 by (inv tys2; inv H; inv H4; auto).
-assert (wf_vtype B1) as wfb1 by (inv tys1; inv H; inv H5; auto).
-assert (wf_vtype B2) as wfb2 by (inv tys2; inv H; inv H5; auto).
-assert (wf_ctype D) as wfd by (inv tys1; auto).
-assert (wf_ctx Γ) as wfctx by (inv orig; inv H; inv H10; auto).
-inv orig. inv H.
-assert (get_op_type Σ1 op = None) as getn1.
-{ destruct (get_op_type Σ1 op) eqn: g. destruct p. 2: reflexivity.
-  eapply h_has_case in H10; eauto. destruct H10 as [c f].
-  rewrite f in f1. discriminate. }
-assert (get_op_type Σ2 op = None) as getn2.
-{ destruct (get_op_type Σ2 op) eqn: g. destruct p. 2: reflexivity.
-  eapply h_has_case in H11; eauto. destruct H11 as [c f].
-  rewrite f in f2. discriminate. }
-assert (sig_subtype Σ (SigU Σ1 op A1 B1)) as ss1.
-{ apply sig_subtype_extend. auto. apply WfSigU; auto. inv H10. assumption. }
-assert (sig_subtype Σ (SigU Σ2 op A2 B2)) as ss2.
-{ apply sig_subtype_extend. auto. apply WfSigU; auto. inv H11. assumption. }
-induction Σ as [ | Σ IH o A B].
-+ eapply WfJudg; auto. eapply WfHeq. auto. exact ss1. exact ss2.
-  - apply TypeH. 2:apply WfSigU. 2:inv H10. 7:apply TypeCasesU. all: auto.
-  - apply TypeH. 2:apply WfSigU. 2:inv H11. 7:apply TypeCasesU. all: auto.
-  - apply HeqSigØ.
-+ eapply WfJudg; auto. eapply WfHeq. auto. exact ss1. exact ss2.
-  - apply TypeH. 2:apply WfSigU. 2:inv H10. 7:apply TypeCasesU. all: auto.
-  - apply TypeH. 2:apply WfSigU. 2:inv H11. 7:apply TypeCasesU. all: auto.
-  - inv H1. eapply HeqSigU.
-    * simpl. destruct (o==op). rewrite e, f1 in H12. discriminate. eauto.
-    * simpl. destruct (o==op). rewrite e, f2 in H16. discriminate. eauto.
-    * assumption.
-    * inv H18. inv H6. inv H8. inv H9.
-      apply IH; auto. 
-      all: apply sig_subtype_extend; auto.
-      all: apply WfSigU; auto. inv H10. auto. inv H11. auto.
-Qed. *)
-
-
-(* Lemma heq_case_extend_structural Σ D Γ Ψ h1 h2 op A B c1 c2:
-  judg Γ Ψ (Heq Σ D h1 h2) ->
-  get_case h1 op = None -> get_case h2 op = None ->
-  judg (CtxU (CtxU Γ A) (TyFun B D)) (hyp_shift Ψ 2 0) (Ceq D c1 c2) ->
-  judg Γ Ψ (Heq (SigU Σ op A B) D (CasesU h1 op c1) (CasesU h2 op c2)).
-Proof.
-intros orig f1 f2 ceq12.
-assert (has_ctype (CtxU (CtxU Γ A) (TyFun B D)) c1 D) as tys1.
-{ inv ceq12. inv H. auto. }
-assert (has_ctype (CtxU (CtxU Γ A) (TyFun B D)) c2 D) as tys2.
-{ inv ceq12. inv H. auto. }
-assert (wf_vtype A) as wfa by (inv tys1; inv H; inv H4; auto).
-assert (wf_vtype B) as wfb by (inv tys1; inv H; inv H5; auto).
-assert (wf_ctype D) as wfd by (inv tys1; auto).
-assert (wf_ctx Γ) as wfctx by (inv orig; inv H; inv H10; auto).
-inv orig. inv H.
-assert (get_op_type Σ1 op = None) as getn1.
-{ destruct (get_op_type Σ1 op) eqn: g. destruct p. 2: reflexivity.
-  eapply h_has_case in H10; eauto. destruct H10 as [c f].
-  rewrite f in f1. discriminate. }
-assert (get_op_type Σ2 op = None) as getn2.
-{ destruct (get_op_type Σ2 op) eqn: g. destruct p. 2: reflexivity.
-  eapply h_has_case in H11; eauto. destruct H11 as [c f].
-  rewrite f in f2. discriminate. }
-assert (sig_subtype (SigU Σ op A B) (SigU Σ1 op A B)) as ss1.
-{ eapply SubtypeSigU. apply sig_subtype_extend. auto. apply WfSigU; auto. 
-  inv H10. auto. simpl. destruct (op==op). reflexivity. destruct n. auto.
-  all: apply vsubtype_refl; auto. }
-assert (sig_subtype (SigU Σ op A B) (SigU Σ2 op A B)) as ss2.
-{ eapply SubtypeSigU. apply sig_subtype_extend. auto. apply WfSigU; auto. 
-  inv H11. auto. simpl. destruct (op==op). reflexivity. destruct n. auto.
-  all: apply vsubtype_refl; auto. }
-assert (get_op_type Σ op = None) as sgetnone.
-{ destruct (get_op_type Σ op) eqn: gs; auto. destruct p.
-  eapply sig_subtype_get_Some in H8; eauto. destruct H8 as [a[b[g]]]. 
-  rewrite g in getn1. discriminate. }
-eapply WfJudg; auto. eapply WfHeq. apply WfSigU; auto. exact ss1. exact ss2.
-- apply TypeH. 2:apply WfSigU. 2:inv H10. 7:apply TypeCasesU. all: auto.
-- apply TypeH. 2:apply WfSigU. 2:inv H11. 7:apply TypeCasesU. all: auto.
-- eapply HeqSigU.
-  * simpl. destruct (op==op). reflexivity. destruct n. auto.
-  * simpl. destruct (op==op). reflexivity. destruct n. auto.
-  * assumption.
-  * eapply heq_case_extend_trivial; eauto. 
-    eapply WfJudg. eapply WfHeq. 2:exact H8. all: eauto.
-Qed. *)
 
 (* ================== Reflexivity, Symmetry, Transitivity ================== *)
 
@@ -374,8 +32,7 @@ destruct orig. destruct H1.
 + apply VeqListCons; eauto.
 + apply VeqFun; eauto. 
 + eapply VeqHandler; eauto. apply csubtype_refl. inv H2. assumption.
-+ apply veq_refl_raw in H1. admit.
-   (* eapply veq_subtype in H1; eauto. inv H1. assumption. *)
++ apply veq_refl_raw in H1. eapply VeqSubtype; eauto.
 }{
 apply WfJudg. apply WfCeq; auto. apply WfHypØ. inv orig. auto.
 destruct orig. destruct H1.
@@ -389,29 +46,26 @@ destruct orig. destruct H1.
 + eapply CeqHandle; eauto.
 + eapply CeqLetRec; eauto.
 + eapply CeqOp; eauto.
-+ apply ceq_refl_raw in H1. admit.
-  (* eapply ceq_subtype in H1; eauto. inv H1. assumption. *)
++ apply ceq_refl_raw in H1. eapply CeqSubtype; eauto.
 }{
-  admit.
-(* apply WfJudg. eapply WfHeq; auto.
+apply WfJudg. eapply WfHeq; auto.
 inv orig. assumption.
 apply sig_subtype_refl. inv orig. assumption.
 apply sig_subtype_refl. inv orig. assumption.
 assumption. assumption. apply WfHypØ. inv orig. assumption.
 destruct orig. destruct H2.
 + eapply HeqSigØ.
-+ assert (get_case (CasesU h op cop) op = Some cop).
-  { simpl. destruct (op==op). auto. destruct n. auto. }
-  eapply HeqSigU; eauto.
-  eapply heq_case_extend_trivial; eauto; inv H0; assumption. *)
++ eapply HeqExtend; eauto.
 }
-Admitted.
+Qed.
 
 
 Lemma veq_sym A Γ Ψ v1 v2 : 
   judg Γ Ψ (Veq A v1 v2) -> judg Γ Ψ (Veq A v2 v1)
 with ceq_sym C Γ Ψ c1 c2 : 
-  judg Γ Ψ (Ceq C c1 c2) -> judg Γ Ψ (Ceq C c2 c1).
+  judg Γ Ψ (Ceq C c1 c2) -> judg Γ Ψ (Ceq C c2 c1)
+with heq_sym Σ D Γ Ψ h1 h2 : 
+  judg Γ Ψ (Heq Σ D h1 h2) -> judg Γ Ψ (Heq Σ D h2 h1).
 Proof.
 {
 intro orig. apply WfJudg. apply WfVeq. all: try (inv orig; inv H; assumption).
@@ -419,29 +73,23 @@ apply VeqSym. auto.
 }{
 intro orig. apply WfJudg. apply WfCeq. all: try (inv orig; inv H; assumption).
 apply CeqSym. auto.
+}{
+intro orig. apply WfJudg. inv orig. inv H.
+eapply WfHeq. 3: exact H8. all: eauto. inv orig. auto.
+apply HeqSym. auto.
 }
 Qed.
-(* 
-Lemma heq_sym Σ D Γ Ψ h1 h2 : 
-  judg Γ Ψ (Heq Σ D h1 h2) -> judg Γ Ψ (Heq Σ D h2 h1).
-Proof.
-induction Σ; intros orig.
-all: apply WfJudg; try (inv orig; assumption).
-+ inv orig. inv H. eapply WfHeq. auto.
-  exact H9. exact H8. all: eauto.
-+ apply HeqSigØ.
-+ inv orig. inv H. eapply WfHeq. auto.
-  exact H9. exact H8. all: eauto. 
-+ inv orig. inv H1. eapply HeqSigU; eauto.
-  apply ceq_sym. auto.
-Qed. *)
 
     
 Lemma veq_trans A Γ Ψ v1 v2 v3:
   judg Γ Ψ (Veq A v1 v2) -> judg Γ Ψ (Veq A v2 v3) -> judg Γ Ψ (Veq A v1 v3)
 
 with  ceq_trans C Γ Ψ c1 c2 c3:
-  judg Γ Ψ (Ceq C c1 c2) -> judg Γ Ψ (Ceq C c2 c3) -> judg Γ Ψ (Ceq C c1 c3).
+  judg Γ Ψ (Ceq C c1 c2) -> judg Γ Ψ (Ceq C c2 c3) -> judg Γ Ψ (Ceq C c1 c3)
+
+with  heq_trans Σ D Γ Ψ h1 h2 h3:
+  judg Γ Ψ (Heq Σ D h1 h2) -> judg Γ Ψ (Heq Σ D h2 h3) -> 
+  judg Γ Ψ (Heq Σ D h1 h3).
 
 Proof.
 {
@@ -456,21 +104,11 @@ intros ceq1 ceq2. apply WfJudg. apply WfCeq.
 + inv ceq2. inv H. auto.
 + inv ceq1. auto.
 + eapply CeqTrans; eauto.
+}{
+intros heq1 heq2. apply WfJudg. 
++ inv heq1. inv H. inv heq2. inv H. eapply WfHeq.
+  4: eauto. 4: eauto. all:eauto.
++ inv heq1. auto.
++ eapply HeqTrans; eauto.
 }
 Qed.
-
-(* 
-Lemma heq_trans Σ D Γ Ψ h1 h2 h3:
-  judg Γ Ψ (Heq Σ D h1 h2) -> judg Γ Ψ (Heq Σ D h2 h3) -> 
-  judg Γ Ψ (Heq Σ D h1 h3).
-{
-intros heq1 heq2. induction Σ.
-+ inv heq1. inv heq2. inv H. inv H2. eapply WfJudg. eapply WfHeq.
-  2: exact H11. 2: exact H16. all: eauto. apply HeqSigØ.
-+ inv heq1. inv heq2. inv H. inv H2. eapply WfJudg. eapply WfHeq.
-  2: exact H11. 2: exact H16. all: eauto. 
-  inv H1. inv H4. eapply HeqSigU; eauto.
-  rewrite H10 in H23. inv H23.
-  eapply ceq_trans; eauto.
-}
-Qed. *)
